Finish correcting proofs

src/Translation.v
@@ -18,17 +18,22 @@ Import UpdateNotations.
 Section translate_pattern.
   Import Pattern.
 
+  Definition translate_props (mode : FilterMode.t) (n : Name.t) props plan :=
+    fold_right (fun '(k, v) => FilterByProperty mode n k v) plan props.
+
   Definition translate_pvertex pv plan : ExecutionPlan.t :=
-    match vlabel pv with
-    | Some l => FilterByLabel Vertices (vname pv) l plan
-    | None => plan
-    end.
+    let plan := match vlabel pv with
+                | Some l => FilterByLabel Vertices (vname pv) l plan
+                | None => plan
+                end
+    in translate_props Vertices (vname pv) (vprops pv) plan.
 
   Definition translate_pedge pe plan : ExecutionPlan.t :=
-    match elabel pe with
-    | Some l => FilterByLabel Edges (ename pe) l plan
-    | None => plan
-    end.
+    let plan := match elabel pe with
+                | Some l => FilterByLabel Edges (ename pe) l plan
+                | None => plan
+                end
+    in translate_props Edges (ename pe) (eprops pe) plan.
 
   Fixpoint translate_pattern' (pi : Pattern.t) : ExecutionPlan.t :=
     match pi with
@@ -36,7 +41,7 @@ Section translate_pattern.
         translate_pvertex pv (ScanVertices (vname pv))
     | Pattern.hop pi pe pv =>
       let mode := 
-        if ((PatternT.type_of Full pi (vname pv)) == (Some Value.GVertexT))
+        if ((PatternT.type_of Full pi (vname pv)) ==b (Some Value.GVertexT))
         then Into else All
       in
       let plan := translate_pattern' pi in
@@ -50,6 +55,12 @@ Section translate_pattern.
     ReturnAll (translate_pattern' pi).
 End translate_pattern.
 
+Lemma translate_props_type mode n props plan :
+  type_of (translate_props mode n props plan) = type_of plan.
+Proof using.
+  induction props as [| [k v] props]; simpls.
+Qed.
+
 Ltac desf_translate_pvertex_pedge :=
   unfold translate_pvertex, translate_pedge in *;
   desf; simpls;
@@ -57,11 +68,17 @@ Ltac desf_translate_pvertex_pedge :=
 
 Lemma translate_pvertex_type pv plan :
   type_of (translate_pvertex pv plan) = type_of plan.
-Proof using. desf_translate_pvertex_pedge. Qed.
+Proof using.
+  desf_translate_pvertex_pedge.
+  all: now rewrite translate_props_type.
+Qed.
 
 Lemma translate_pedge_type pe plan :
   type_of (translate_pedge pe plan) = type_of plan.
-Proof using. desf_translate_pvertex_pedge. Qed.
+Proof using.
+  desf_translate_pvertex_pedge.
+  all: now rewrite translate_props_type.
+Qed.
 
 Theorem translate_pattern'_type pi (Hwf : PatternT.wfT pi) :
   type_of (translate_pattern' pi) = PatternT.type_of Full pi.
@@ -84,20 +101,60 @@ Proof using.
   now rewrite PatternT.explicit_projT_type_of.
 Qed.
 
+Lemma translate_props_wf mode n props plan
+  (Htype : match mode with
+           | Vertices => type_of plan n = Some Value.GVertexT
+           | Edges => type_of plan n = Some Value.GEdgeT
+           end)
+  (Hwf : ExecutionPlan.wf plan) :
+    ExecutionPlan.wf (translate_props mode n props plan).
+Proof using.
+  destruct mode.
+  all: induction props as [| [k v] props]; simpls.
+  all: unnw; intuition.
+  all: now rewrite translate_props_type.
+Qed.
+
+Lemma translate_pvertex_wf pv plan
+  (Htype : type_of plan (Pattern.vname pv) = Some Value.GVertexT)
+  (Hwf : ExecutionPlan.wf plan) :
+    ExecutionPlan.wf (translate_pvertex pv plan).
+Proof using.
+  unfold translate_pvertex; desf.
+  all: apply translate_props_wf; simpls.
+Qed.
+
+Lemma translate_pedge_wf pe plan
+  (Htype : type_of plan (Pattern.ename pe) = Some Value.GEdgeT)
+  (Hwf : ExecutionPlan.wf plan) :
+    ExecutionPlan.wf (translate_pedge pe plan).
+Proof using.
+  unfold translate_pedge; desf.
+  all: apply translate_props_wf; simpls.
+Qed.
+
 Theorem translate_pattern'_wf pi (Hwf : PatternT.wfT pi) :
   ExecutionPlan.wf (translate_pattern' pi).
 Proof using.
   induction pi; simpls.
-  all: inv Hwf.
-  all: unfold translate_pvertex, translate_pedge.
-  all: desf; simpls; splits; auto.
-  all: normalize_bool.
-  all: desf_unfold_pat.
-  all: try contradiction.
-  all: try congruence.
-  all: try rewrite translate_pattern'_type; auto.
+  { apply translate_pvertex_wf; simpls.
+    apply PartialMap.update_eq. }
+  inv Hwf.
+  apply translate_pvertex_wf.
+  { rewrite translate_pedge_type.
+    case equiv_decbP; intros Heq; simpls.
+    all: rewrite translate_pattern'_type by assumption.
+    all: apply PartialMap.update_eq. }
+  apply translate_pedge_wf.
+  { simpls. rewrite PartialMap.update_neq by assumption.
+    now rewrite PartialMap.update_eq. }
+  simpls.
+  case equiv_decbP; intros Heq; unnw.
+  all: rewrite translate_pattern'_type by assumption.
+  all: splits; auto.
   all: try apply PatternT.last__dom_vertices.
-  all: intros contra; eapply PatternT.last_neq_pe; eauto.
+  all: try now (intros contra; eapply PatternT.last_neq_pe; eauto).
+  desf.
 Qed.
 
 Theorem translate_pattern_wf pi (Hwf : PatternT.wfT pi) :
@@ -107,9 +164,218 @@ Proof using.
   now apply translate_pattern'_wf.
 Qed.
 
-Module EvalQueryImpl (S : ExecutionPlan.Spec) : EvalQuery.Spec.
+Module EvalPvertexPedge (S : ExecutionPlan.Spec).
   Module EvalPlanImpl := EvalPlan S.
   Import S.
+  Import EvalPlanImpl.
+
+  Lemma eval_translate_props_reduce graph mode n props plan table'
+    (Hres : eval graph (translate_props mode n props plan) = Some table') :
+      exists table, eval graph plan = Some table.
+  Proof using.
+    gen_dep table'.
+    induction props as [| [k v] props]; intros.
+    { eauto 2. }
+    simpl in Hres.
+    eval_operation_reduce in Hres.
+    eauto using IHprops.
+  Qed.
+
+  Lemma eval_translate_pvertex_reduce graph pv plan table'
+    (Hres : eval graph (translate_pvertex pv plan) = Some table') :
+      exists table, eval graph plan = Some table.
+  Proof.
+    unfold translate_pvertex in *.
+    apply eval_translate_props_reduce in Hres as [table'' Hres].
+    desf; simpls.
+    1: eval_operation_reduce in Hres.
+    all: eauto 2.
+  Qed.
+
+  Lemma eval_translate_pedge_reduce graph pe plan table'
+    (Hres : eval graph (translate_pedge pe plan) = Some table') :
+      exists table, eval graph plan = Some table.
+  Proof.
+    unfold translate_pedge in *.
+    apply eval_translate_props_reduce in Hres as [table'' Hres].
+    desf; simpls.
+    1: eval_operation_reduce in Hres.
+    all: eauto 2.
+  Qed.
+
+
+  Lemma eval_translate_props_spec graph mode n props plan table table' r
+    (Hres : eval graph plan = Some table)
+    (Hres' : eval graph (translate_props mode n props plan) = Some table')
+    (HIn : In r table)
+    (H : match mode with
+         | Vertices => exists v,
+             << Hval : r n = Some (Value.GVertex v) >> /\
+             << Hprops : Forall (fun '(k, val) => get_vprop graph k v = Some val) props >>
+         | Edges => exists e,
+             << Hval : r n = Some (Value.GEdge e) >> /\
+             << Hprops : Forall (fun '(k, val) => get_eprop graph k e = Some val) props >>
+         end) :
+      In r table'.
+  Proof using.
+    gen_dep table'.
+    induction props as [| [k val] props]; ins.
+    { congruence. }
+
+    destruct mode; desc.
+    all: assert (Hprop := Hprops).
+    all: apply Forall_inv in Hprop.
+    all: apply Forall_inv_tail in Hprops.
+
+    all: eval_operation_reduce in Hres'.
+    { eauto using filter_vertices_by_property_spec. }
+    { eauto using filter_edges_by_property_spec. }
+  Qed.
+
+  Lemma eval_translate_pvertex_spec graph pv plan table table' r v
+    (Hres : eval graph plan = Some table)
+    (Hres' : eval graph (translate_pvertex pv plan) = Some table')
+    (HIn : In r table)
+    (Hval : r (Pattern.vname pv) = Some (Value.GVertex v))
+    (Hprops : Forall (fun '(k, val) => get_vprop graph k v = Some val)
+                     (Pattern.vprops pv))
+    (Hlabel : match Pattern.vlabel pv with
+              | Some l => In l (vlabels graph v)
+              | None => True
+              end) :
+      In r table'.
+  Proof.
+    unfold translate_pvertex in *. simpls.
+    assert (Hres_filter := Hres').
+    apply eval_translate_props_reduce in Hres_filter as [table'' Hres_filter].
+    eapply eval_translate_props_spec; eauto.
+    2: { simpl. eauto. }
+
+    destruct (Pattern.vlabel pv).
+    2: { congruence. }
+
+    simpl in Hres_filter.
+    eval_operation_reduce in Hres_filter.
+    eapply filter_vertices_by_label_spec; eauto.
+    assert (table = table0) by congruence.
+    now subst.
+  Qed.
+
+  Lemma eval_translate_pedge_spec graph pe plan table table' r e
+    (Hres : eval graph plan = Some table)
+    (Hres' : eval graph (translate_pedge pe plan) = Some table')
+    (HIn : In r table)
+    (Hval : r (Pattern.ename pe) = Some (Value.GEdge e))
+    (Hprops : Forall (fun '(k, val) => get_eprop graph k e = Some val)
+                     (Pattern.eprops pe))
+    (Hlabel : match Pattern.elabel pe with
+              | Some l => elabel graph e = l
+              | None => True
+              end) :
+      In r table'.
+  Proof.
+    unfold translate_pedge in *. simpls.
+    assert (Hres_filter := Hres').
+    apply eval_translate_props_reduce in Hres_filter as [table'' Hres_filter].
+    eapply eval_translate_props_spec; eauto.
+    2: { simpl. eauto. }
+
+    destruct (Pattern.elabel pe).
+    2: { congruence. }
+
+    simpl in Hres_filter.
+    eval_operation_reduce in Hres_filter.
+    eapply filter_edges_by_label_spec; eauto.
+    assert (table = table0) by congruence.
+    now subst.
+  Qed.
+
+
+  Lemma eval_translate_props_spec' graph mode n props plan table table' r
+    (Hres : eval graph plan = Some table)
+    (Hres' : eval graph (translate_props mode n props plan) = Some table')
+    (HIn : In r table') :
+      In r table /\ (props = [] \/
+        match mode with
+        | Vertices => exists v,
+            << Hval : r n = Some (Value.GVertex v) >> /\
+            << Hprops : Forall (fun '(k, val) => get_vprop graph k v = Some val) props >>
+        | Edges => exists e,
+            << Hval : r n = Some (Value.GEdge e) >> /\
+            << Hprops : Forall (fun '(k, val) => get_eprop graph k e = Some val) props >>
+        end).
+  Proof.
+    gen_dep table'.
+    induction props as [| [k val] props]; ins.
+    { split.
+      { congruence. }
+      now left. }
+    eval_operation_reduce in Hres' eqn:Hres_filter.
+    destruct mode;
+    [ eapply filter_vertices_by_property_spec' in Hres_filter |
+      eapply filter_edges_by_property_spec' in Hres_filter ]; eauto.
+    all: desc; unnw.
+    all: edestruct IHprops; eauto 1; desf.
+    all: eauto 10 using Forall_cons.
+  Qed.
+
+  Lemma eval_translate_pvertex_spec' graph pv plan table table' r
+    (Hres : eval graph plan = Some table)
+    (Hres' : eval graph (translate_pvertex pv plan) = Some table')
+    (HIn : In r table') :
+      << HIn : In r table >> /\
+      forall v, r (Pattern.vname pv) = Some (Value.GVertex v) ->
+        << Hlabel : match Pattern.vlabel pv with
+                    | Some l => In l (vlabels graph v)
+                    | None => True
+                    end >> /\
+        << Hprops : Forall (fun '(k, val) => get_vprop graph k v = Some val)
+                          (Pattern.vprops pv) >>.
+  Proof.
+    unfold translate_pvertex in *.
+    assert (Hres'' := Hres').
+    eapply eval_translate_props_reduce in Hres'' as [table'' Hres'']; eauto.
+    eapply eval_translate_props_spec' in Hres'; eauto.
+    all: desf; simpls.
+    all: try eval_operation_reduce in Hres'' eqn:Hres_filter.
+    all: try (eapply filter_vertices_by_label_spec' in Hres_filter; eauto).
+    all: desf; unnw; intuition.
+    all: try assert (v = v0) by congruence; subst.
+    all: auto.
+    all: now rewrite Hres'0.
+  Qed.
+
+  Lemma eval_translate_pedge_spec' graph pe plan table table' r
+    (Hres : eval graph plan = Some table)
+    (Hres' : eval graph (translate_pedge pe plan) = Some table')
+    (HIn : In r table') :
+      << HIn : In r table >> /\
+      forall e, r (Pattern.ename pe) = Some (Value.GEdge e) ->
+        << Hlabel : match Pattern.elabel pe with
+                    | Some l => elabel graph e = l
+                    | None => True
+                    end >> /\
+        << Hprops : Forall (fun '(k, val) => get_eprop graph k e = Some val)
+                          (Pattern.eprops pe) >>.
+  Proof.
+    unfold translate_pedge in *.
+    assert (Hres'' := Hres').
+    eapply eval_translate_props_reduce in Hres'' as [table'' Hres'']; eauto.
+    eapply eval_translate_props_spec' in Hres'; eauto.
+    all: desf; simpls.
+    all: try eval_operation_reduce in Hres'' eqn:Hres_filter.
+    all: try (eapply filter_edges_by_label_spec' in Hres_filter; eauto).
+    all: desf; unnw; intuition.
+    all: try assert (e = e0) by congruence; subst.
+    all: auto.
+    all: now rewrite Hres'0.
+  Qed.
+End EvalPvertexPedge.
+
+Module EvalQueryImpl (S : ExecutionPlan.Spec) : EvalQuery.Spec.
+  Module EvalPvertexPedgeImpl := EvalPvertexPedge S.
+  Import S.
+  Import EvalPvertexPedgeImpl.
   Import EvalPlanImpl.
 
   Definition eval_match_clause (graph : PropertyGraph.t) (pi : Pattern.t) : option BindingTable.t :=
@@ -135,17 +401,14 @@ Module EvalQueryImpl (S : ExecutionPlan.Spec) : EvalQuery.Spec.
     auto using translate_pattern_wf.
   Qed.
 
-  Ltac desf_match_result Hres :=
-    unfold eval_match_clause in Hres; simpls;
-    desf_translate_pvertex_pedge;
-    unfold option_bind in *; desf.
-
   Theorem eval_translate_pattern'_reduce graph pi pe pv table'
     (Hres : eval graph (translate_pattern' (Pattern.hop pi pe pv)) = Some table') :
       exists table, eval graph (translate_pattern' pi) = Some table.
   Proof using.
-    desf_match_result Hres.
-    all: eauto.
+    simpls.
+    apply eval_translate_pvertex_reduce in Hres as [table'' Hres].
+    apply eval_translate_pedge_reduce in Hres as [table Hres].
+    simpls. eval_operation_reduce in Hres. eauto 2.
   Qed.
 
   Definition expansion_of_by_hop' graph r' r mode v_from e v_to pi pe pv :=
@@ -208,35 +471,34 @@ Module EvalQueryImpl (S : ExecutionPlan.Spec) : EvalQuery.Spec.
     all: destruct Hpv.
     all: try destruct Hpe.
 
-    { all: desf_match_result Hres.
-      1: eapply filter_vertices_by_label_spec; eauto.
-      { apply PartialMap.update_eq. }
-      all: eauto using scan_vertices_spec. }
-
-    desf; simpls.
-
-    all: desf_match_result Hres.
-    
-    all: repeat match goal with
-         | [H : filter_by_label Vertices _ _ _ _ = _ |- _ ] =>
-            eapply filter_vertices_by_label_spec; eauto; clear H
-         | [H : filter_by_label Edges _ _ _ _ = _ |- _ ] =>
-            eapply filter_edges_by_label_spec; eauto; clear H
-         end.
-
-    all: unfold_update_with_mode.
+    all: assert (Hres' := Hres).
+    all: apply eval_translate_pvertex_reduce in Hres' as [table Hres'].
+    all: eapply eval_translate_pvertex_spec; eauto.
     all: try apply PartialMap.update_eq.
-    all: try (rewrite PartialMap.update_neq; auto).
-    all: try apply PartialMap.update_eq.
-    
-    all: match goal with 
-         | [H : expand Into _ _ _ _ _ _ = _ |- _ ] =>
-            apply matches_hop_Into in Hmatch; eauto
-         | [H : expand All _ _ _ _ _ _ = _ |- _ ] =>
-            apply matches_hop_All in Hmatch; eauto
-         end.
-    all: desf.
-    all: eapply expand_spec; eauto.
+    all: try now (desf; auto).
+    { eauto using scan_vertices_spec. }
+
+    assert (Hres'' := Hres').
+    apply eval_translate_pedge_reduce in Hres'' as [table'' Hres''].
+
+    eapply eval_translate_pedge_spec; eauto.
+    2: { unfold update_with_mode_hop.
+         rewrite PartialMap.update_neq by assumption.
+         apply PartialMap.update_eq. }
+    2: { desf; auto. }
+
+    simpl in Hres''.
+    eval_operation_reduce in Hres'' eqn:Hres_expand.
+    eapply expand_spec; eauto.
+
+    case equiv_decbP; intros Heq.
+    1: eapply matches_hop_Into in Hmatch; eauto.
+    2: eapply matches_hop_All in Hmatch; eauto.
+    3: now desf.
+
+    all: desc; unfold expansion_of_by_hop in *.
+    all: assert (r = r0) by eauto using Path.matches_two_records.
+    all: now subst.
   Qed.
 
   Theorem match_clause_spec graph path pi table' r'
@@ -246,7 +508,8 @@ Module EvalQueryImpl (S : ExecutionPlan.Spec) : EvalQuery.Spec.
     (Hmatch : Path.matches Explicit graph r' path pi) :
       In r' table'.
   Proof using.
-    desf_match_result Hres.
+    unfold eval_match_clause, translate_pattern in *; simpls.
+    eval_operation_reduce in Hres eqn:Hres_return.
     assert (Hmatch' := Hmatch).
     eapply Path.matches_explicit_exists_proj in Hmatch' as [r ?]; auto.
     erewrite Path.matches_both_modes with (r := r'); eauto.
@@ -260,6 +523,8 @@ Module EvalQueryImpl (S : ExecutionPlan.Spec) : EvalQuery.Spec.
     (Hdom : Path.matches Full graph r path pi)
     (Hvlabel : forall l : label, Pattern.vlabel pv = Some l -> In l (vlabels graph v_to))
     (Helabel : forall l : label, Pattern.elabel pe = Some l -> elabel graph e = l)
+    (Hvprops : Forall (fun '(k, val) => get_vprop graph k v_to = Some val) (Pattern.vprops pv))
+    (Heprops : Forall (fun '(k, val) => get_eprop graph k e = Some val) (Pattern.eprops pe))
     (Hexp : expansion_of_by_hop' graph r' r mode v_from e v_to pi pe pv) :
       Path.matches Full graph r' (Path.hop path e v_to) (Pattern.hop pi pe pv).
   Proof using.
@@ -290,34 +555,55 @@ Module EvalQueryImpl (S : ExecutionPlan.Spec) : EvalQuery.Spec.
     gen_dep Hres r' table'.
     induction pi; ins.
     all: inv Hwf.
-    all: desf_match_result Hres.
-    all: repeat match goal with
-         | [H : filter_by_label Vertices _ _ _ _ = _ |- _ ] =>
-            eapply filter_vertices_by_label_spec' in H; try eassumption; desf
-         | [H : filter_by_label Edges _ _ _ _ = _ |- _ ] =>
-            eapply filter_edges_by_label_spec' in H; try eassumption; desf
-         end.
-    all: try match goal with
-          | [H : scan_vertices _ _ = _ |- _ ] =>
-             eapply scan_vertices_spec' in H; try eassumption; desf
-          end.
-    all: repeat match goal with
-         | [H : expand _ _ _ _ _ _ _ = _ |- _ ] =>
-            eapply expand_spec' in H; try eassumption; desf
-         end.
-    all: try edestruct IHpi as [path ?]; eauto.
+    
+    all: assert (Hres' := Hres).
+    all: apply eval_translate_pvertex_reduce in Hres' as [table'' Hres'].
+    all: eapply eval_translate_pvertex_spec' in Hres; eauto.
+    all: desc.
+    
+    { eapply scan_vertices_spec' in Hres'.
+      2: eassumption.
+      desc. subst.
+      edestruct Hres0.
+      { apply PartialMap.update_eq. }
+      exists (Path.start v).
+      lift_to_update_with_mode.
+      do 2 constructor; auto.
+      ins. desf. }
 
-    all: unfold expansion_of_by_hop, expansion_of in *; desf.
-    1-2: eexists (Path.start _).
-    all: try eexists (Path.hop path _ _).
+    assert (Hres'' := Hres').
+    eapply eval_translate_pedge_reduce in Hres'' as [table''' Hres''].
+    eapply eval_translate_pedge_spec' in Hres'; eauto; desc.
+    simpl in Hres''.
+    eval_operation_reduce in Hres'' eqn:Hres_expand.
+    eapply expand_spec' in Hres_expand; eauto; desc.
+    unfold expansion_of_by_hop, expansion_of, expansion_of' in *; desc.
 
-    1-2: lift_to_update_with_mode.
-    1-2: do 2 constructor; auto.
+    edestruct IHpi with (table' := table) as [p IH]; eauto.
+    exists (Path.hop p e v_to).
 
-    all: try eapply matches_expansion_of; eauto.
-    all: try unfold expansion_of_by_hop, expansion_of, expansion_of' in *.
-    all: unfold_update_with_mode.
-    all: ins; desf_unfold_pat.
+    erewrite Path.matches_full_last in Hval_from by eauto.
+    injection Hval_from as Hval_from; subst.
+
+    specialize (Hres0 v_to). specialize (Hres'0 e).
+    destruct Hres0.
+    { apply PartialMap.update_eq. }
+    destruct Hres'0.
+    { rewrite PartialMap.update_neq by auto.
+      apply PartialMap.update_eq. }
+    unnw.
+
+    lift_to_update_with_mode.
+    constructor; auto.
+    1-2: constructor; auto.
+    all: try now (intros ? ?; desf).
+    { unfold Path.matches_direction in *.
+      destruct (Pattern.edir pe).
+      3: destruct Hdir.
+      all: edestruct ends_In; eauto. }
+    
+    destruct (equiv_decbP (PatternT.type_of Full pi (Pattern.vname pv))
+                          (Some Value.GVertexT)); auto.
   Qed.
 
   Theorem match_clause_spec' graph pi table' r'
@@ -327,7 +613,8 @@ Module EvalQueryImpl (S : ExecutionPlan.Spec) : EvalQuery.Spec.
     (HIn : In r' table') :
       exists path, Path.matches Explicit graph r' path pi.
   Proof using.
-    desf_match_result Hres.
+    unfold eval_match_clause, translate_pattern in *; simpls.
+    eval_operation_reduce in Hres eqn:Hres_return.
     eapply return_all_spec' in HIn; eauto; desf.
     edestruct eval_translate_pattern'_spec'; eauto.
     eexists.
